ArkLib/ProofSystem/Component/RandomQuery.lean
@@ -1,0 +1,170 @@
+/-
+Copyright (c) 2025 ArkLib Contributors. All rights reserved.
+Released under Apache 2.0 license as described in the file LICENSE.
+Authors: Quang Dao
+-/
+import ArkLib.OracleReduction.Security.Basic
+
+/-!
+# Building blocks for oracle reductions - RandomQuery
+
+We describe common (1-message) protocols that serve as building blocks for constructing oracle
+reductions. Each of these components is an oracle reduction with a single message (from prover or
+from verifier), and does a minimal amount of computation.
+
+Assume that the beginning data consists of `Statement`, `OStatement`, and `Witness`, and a
+relation `rel : Statement → OStatement → Witness → Prop`.
+-/
+
+open OracleSpec OracleComp OracleQuery
+
+namespace RandomQuery
+
+open OracleInterface
+
+/-!
+3. - There is no witness nor public statement. There are two `OStatement`s, `a` and `b`,
+     of the same type. The relation is `a = b`.
+   - The verifier samples random `q : OracleInterface.Query` for that type
+   and sends it to the prover.
+   - The verifier does not do any checks.
+   - The final relation is that `a` and `b` are equal at that query.
+-/
+
+variable {ι : Type} (oSpec : OracleSpec ι) (OStatement : Type) [OracleInterface OStatement]
+  [inst : VCVCompatible (Query OStatement)]
+
+@[reducible]
+def pSpec : ProtocolSpec 1 := ![(.V_to_P, Query OStatement)]
+
+instance : ∀ i, OracleInterface ((pSpec OStatement).Message i) | ⟨0, h⟩ => nomatch h
+@[reducible, simp] instance : ∀ i, VCVCompatible ((pSpec OStatement).Challenge i)
+  | ⟨0, _⟩ => by dsimp [pSpec, ProtocolSpec.Challenge]; exact inst
+
+/--
+The prover is trivial: it has no messages to send.  It only receives the verifier's challenge `q`.
+We keep track of `(a, b)` in the prover's state, along with the single random query `q`.
+-/
+def prover : OracleProver (pSpec OStatement) oSpec Unit Unit
+    (Query OStatement) Unit
+    (fun _ : Fin 2 => OStatement) (fun _ : Fin 2 => OStatement) where
+
+  PrvState
+  | 0 => OStatement × OStatement
+  | 1 => OStatement × OStatement × (Query OStatement)
+
+  input := fun ⟨(), oracles⟩ () => (oracles 0, oracles 1)
+
+  sendMessage | ⟨0, h⟩ => nomatch h
+
+  receiveChallenge | ⟨0, _⟩ => fun (a, b) q => (a, b, q)
+
+  output := fun (a, b, q) => ((q, ![a, b]), ())
+
+/--
+The verifier queries both `a` and `b` at the random point `q`.
+We check `OracleInterface.oracle a q = OracleInterface.oracle b q`.
+-/
+def verifier : OracleVerifier (pSpec OStatement) oSpec Unit (Query OStatement)
+    (fun _ : Fin 2 => OStatement) (fun _ : Fin 2 => OStatement) where
+
+  verify := fun _ chal => do
+    let q : OracleInterface.Query OStatement := chal ⟨0, rfl⟩
+    -- let resp ← liftM <| query
+    --   (spec := (oSpec ++ₒ ([fun x ↦ OStatement]ₒ ++ₒ [(pSpec OStatement).Message]ₒ)))
+    --   (Sum.inr <| Sum.inl (0 : Fin 2)) q
+    pure q
+
+  embed := Function.Embedding.inl
+
+  hEq := by simp
+
+/--
+Combine the trivial prover and this verifier to form the oracle reduction:
+the input oracles are `(a, b)`, and the output oracles are the same `(a, b)`.
+-/
+def oracleReduction :
+  OracleReduction (pSpec OStatement) oSpec Unit Unit
+    (Query OStatement) Unit
+    (fun _ : Fin 2 => OStatement) (fun _ : Fin 2 => OStatement) where
+  prover := prover oSpec OStatement
+  verifier := verifier oSpec OStatement
+
+@[reducible]
+def relIn : (Unit × (∀ _ : Fin 2, OStatement)) → Unit → Prop := fun ⟨(), oracles⟩ () =>
+  oracles 0 = oracles 1
+
+/--
+The final relation states that if the verifier's single query was `q`, then
+`a` and `b` agree on that `q`, i.e. `OracleInterface.oracle a q = OracleInterface.oracle b q`.
+-/
+def relOut : ((Query OStatement) × (∀ _ : Fin 2, OStatement)) → Unit → Prop :=
+  fun ⟨q, oStmt⟩ () => OracleInterface.oracle (oStmt 0) q = OracleInterface.oracle (oStmt 1) q
+
+variable [oSpec.FiniteRange]
+
+theorem completeness : OracleReduction.perfectCompleteness
+    (relIn OStatement)
+    (relOut OStatement)
+    (oracleReduction oSpec OStatement) := by
+  sorry
+
+-- def langIn : Set (Unit × (∀ _ : Fin 2, OStatement)) := setOf fun ⟨(), oracles⟩ =>
+--   oracles 0 = oracles 1
+
+-- def langOut : Set ((Query OStatement) × (∀ _ : Fin 2, OStatement)) := setOf fun ⟨q, oracles⟩ =>
+--   OracleInterface.oracle (oracles 0) q = OracleInterface.oracle (oracles 1) q
+
+def stateFunction : (verifier oSpec OStatement).StateFunction (pSpec OStatement) oSpec
+    (relIn OStatement).language (relOut OStatement).language where
+  toFun
+  | 0 => fun ⟨_, oracles⟩ _ => oracles 0 = oracles 1
+  | 1 => fun ⟨_, oracles⟩ chal =>
+    let q : Query OStatement := by simpa [pSpec] using chal ⟨0, by aesop⟩
+    OracleInterface.oracle (oracles 0) q = OracleInterface.oracle (oracles 1) q
+  toFun_empty := fun stmt hStmt => by simp_all [relIn, Function.language]
+  toFun_next := fun i hDir ⟨stmt, oStmt⟩ tr h => by simp_all
+  toFun_full := fun ⟨stmt, oStmt⟩ tr h => by
+    simp_all [relOut, Function.language]
+    intro a b hSupp
+    simp [Verifier.run, OracleVerifier.toVerifier, verifier] at hSupp
+    simp [hSupp.1, hSupp.2, h]
+
+/-- The extractor is trivial since the output witness is `Unit`. -/
+def extractor : RBRExtractor (pSpec OStatement) oSpec
+    (Unit × (∀ _ : Fin 2, OStatement)) Unit :=
+  fun _ _ _ _ => ()
+
+-- The key fact governing the soundness of this reduction is a property of the form
+-- `∀ a b : OStatement, a ≠ b → #{q | OracleInterface.oracle a q = OracleInterface.oracle b q} ≤ d`.
+-- In other words, the oracle instance has distance at most `d`.
+
+variable [Fintype (Query OStatement)] [DecidableEq (Response OStatement)]
+
+instance : Fintype ((pSpec OStatement).Challenge ⟨0, by simp⟩) := by
+  dsimp [pSpec, ProtocolSpec.Challenge]; infer_instance
+
+open NNReal
+
+theorem rbr_knowledge_soundness {d : ℕ} (h : OracleInterface.distanceLE OStatement d) :
+    (verifier oSpec OStatement).rbrKnowledgeSoundness
+      (relIn OStatement)
+      (relOut OStatement)
+      (fun _ => (d : ℝ≥0) / (Fintype.card (Query OStatement) : ℝ≥0)) := by
+  unfold OracleVerifier.rbrKnowledgeSoundness Verifier.rbrKnowledgeSoundness
+  refine ⟨stateFunction oSpec OStatement, extractor oSpec OStatement, ?_⟩
+  intro ⟨_, oracles⟩ _ rbrP i
+  have : i = ⟨0, by simp⟩ := by aesop
+  subst i
+  dsimp at oracles
+  simp [Prover.runWithLogToRound, Prover.runToRound, stateFunction]
+  classical
+  unfold Function.comp
+  simp [probEvent_liftM_eq_mul_inv, ProtocolSpec.Transcript.snoc, Fin.snoc, default]
+  rw [div_eq_mul_inv]
+  gcongr
+  simp [Finset.filter_and]
+  split_ifs with hOracles <;> simp
+  exact h (oracles 0) (oracles 1) hOracles
+
+end RandomQuery
